src/Std/Tactic/BVDecide/LRAT/Checker.lean
@@ -6,10 +6,11 @@ Authors: Henrik Böving
 module
 
 prelude
-public import Std.Tactic.BVDecide.LRAT.Internal.Convert
-public import Std.Tactic.BVDecide.LRAT.Internal.LRATCheckerSound
-public import Std.Tactic.BVDecide.LRAT.Internal.CompactLRATChecker
-import Std.Tactic.BVDecide.LRAT.Internal.CompactLRATCheckerSound
+public import Std.Tactic.BVDecide.LRAT.NewInternal.Checker
+--public import Std.Tactic.BVDecide.LRAT.Internal.Convert
+--public import Std.Tactic.BVDecide.LRAT.Internal.LRATCheckerSound
+--public import Std.Tactic.BVDecide.LRAT.Internal.CompactLRATChecker
+--import Std.Tactic.BVDecide.LRAT.Internal.CompactLRATCheckerSound
 
 @[expose] public section
 
@@ -23,29 +24,31 @@ open Std.Sat
 namespace Std.Tactic.BVDecide
 namespace LRAT
 
-open Std.Tactic.BVDecide.LRAT.Internal
+open Std.Tactic.BVDecide.LRAT
 /--
 Check whether `lratProof` is a valid LRAT certificate for the unsatisfiability of `cnf`.
 -/
 def check (lratProof : Array IntAction) (cnf : CNF Nat) : Bool :=
-  let internalFormula := CNF.convertLRAT cnf
-  let checkerResult := compactLratChecker internalFormula lratProof
-  checkerResult = .success
+  NewInternal.check cnf lratProof
+  --let internalFormula := CNF.convertLRAT cnf
+  --let checkerResult := compactLratChecker internalFormula lratProof
+  --checkerResult = .success
 
-open Std.Tactic.BVDecide.LRAT.Internal in
+--open Std.Tactic.BVDecide.LRAT.Internal in
 /--
 If the `check` functions succeeds on `lratProof` and `cnf` then the `cnf` is unsatisfiable.
 -/
 theorem check_sound (lratProof : Array IntAction) (cnf : CNF Nat) :
     check lratProof cnf → cnf.Unsat := by
-  intro h1
-  apply CNF.unsat_of_convertLRAT_unsat
-  unfold check at h1
-  simp at h1
-  apply compactLratChecker_sound (proof := lratProof)
-  · apply CNF.convertLRAT_readyForRupAdd
-  · apply CNF.convertLRAT_readyForRatAdd
-  · assumption
+  sorry
+  --intro h1
+  --apply CNF.unsat_of_convertLRAT_unsat
+  --unfold check at h1
+  --simp at h1
+  --apply compactLratChecker_sound (proof := lratProof)
+  --· apply CNF.convertLRAT_readyForRupAdd
+  --· apply CNF.convertLRAT_readyForRatAdd
+  --· assumption
 
 end LRAT
 end Std.Tactic.BVDecide
