src/Std/Tactic/BVDecide/LRAT/NewInternal/Checker.lean
@@ -1,0 +1,132 @@
+/-
+Copyright (c) 2026 Lean FRO, LLC. All rights reserved.
+Released under Apache 2.0 license as described in the file LICENSE.
+Authors: Henrik Böving
+-/
+module
+
+prelude
+public import Std.Sat.CNF.Basic
+public import Std.Data.HashMap
+public import Std.Tactic.BVDecide.LRAT.Actions
+import Init.Omega
+
+public section
+
+namespace Std.Tactic.BVDecide.LRAT.NewInternal
+
+open Std.Sat
+
+structure Pos where
+  val : Nat
+  hpos : 0 < val
+
+instance : Inhabited Pos where
+  default := { val := 1, hpos := by omega }
+
+structure State where
+  formula : Array (Option (CNF.Clause Pos))
+
+def State.delete (s : State) (ids : Array Nat) : State :=
+  ids.foldl (init := s) fun s idx =>
+    let ⟨clauses⟩ := s
+    -- TODO: unsound
+    ⟨clauses.setIfInBounds (idx - 1) none⟩
+
+def State.add (s : State) (clause : CNF.Clause Pos) : State :=
+  { s with formula := s.formula.push (some clause) }
+
+structure Assignment where
+  assign : Std.HashMap Nat Bool := {}
+
+@[inline]
+def Assignment.get? (a : Assignment) (lit : Nat) : Option Bool :=
+  a.assign[lit]?
+
+@[inline]
+def Assignment.insert (a : Assignment) (lit : Nat) (b : Bool) : Assignment :=
+  { a with assign := a.assign.insert lit b }
+
+def State.checkRup (s : State) (clause : CNF.Clause Pos) (rupHints : Array Nat) : Bool := Id.run do
+  --dbg_trace s!"Preparing propagation of {clause.literals.map fun (a, p) => (a.1, p)} into {rupHints.map fun idx => s.formula[idx-1]!.map (·.literals.map fun (a, p) => (a.1, p))}"
+  let some assignment := prepareAssignment clause | return true
+  go assignment rupHints 0
+where
+  prepareAssignment (clause : CNF.Clause Pos) : Option Assignment := Id.run do
+    let mut assign := Assignment.mk {}
+    -- TODO: iterator over clauses
+    for (atom, pol) in clause.literals do
+      if let some value := assign.get? atom.val then
+        if value == pol then
+          continue
+        else
+          return none
+      else
+        assign := assign.insert atom.val !pol
+    return some assign
+
+  go (assign : Assignment) (rupHints : Array Nat) (idx : Nat) : Bool := Id.run do
+    if h : idx < rupHints.size then
+      let hint := rupHints[idx]
+      let some (some hintClause) := s.formula[hint - 1]? | return false
+      let mut unit : Option Nat := none
+      let mut assign := assign
+      for (atom, pol) in clause.literals do
+        if let some value := assign.get? atom.val then
+          if value == pol then
+            if unit == some atom.val then
+              continue
+            else
+              return go assign rupHints (idx + 1)
+          else
+            continue
+        else
+          if unit.isSome then
+            return false
+          else
+            unit := some atom.val
+          assign := assign.insert atom.val pol
+      if unit.isNone then
+        return true
+      else
+        return go assign rupHints (idx + 1)
+    else
+      return false
+
+def State.checkEmpty (s : State) (rupHints : Array Nat) : Bool :=
+  s.checkRup .empty rupHints
+
+def check (formula : CNF Nat) (proof : Array IntAction) : Bool :=
+  let state := { formula := convertFormula formula }
+  go state proof 0
+where
+  go (state : State) (proof : Array IntAction) (idx : Nat) : Bool :=
+    if h : idx < proof.size then
+      let step := proof[idx]
+      match step with
+      | .addEmpty id rupHints => state.checkEmpty rupHints
+      | .addRup id clause rupHints =>
+        let clause := convertClause clause
+        if state.checkRup clause rupHints then
+          go (state.add clause) proof (idx + 1)
+        else
+          false
+      | .addRat .. => false -- TODO
+      | .del ids => go (state.delete ids) proof (idx + 1)
+    else
+      false
+
+  convertClause (clause : Array Int) : CNF.Clause Pos :=
+    ⟨clause.toList.filterMap fun int =>
+      if int > 0 then
+        some (⟨int.natAbs, sorry⟩, true)
+      else if int < 0 then
+        some (⟨int.natAbs, sorry⟩, false)
+      else
+        none
+    ⟩
+
+  convertFormula (cnf : CNF Nat) : Array (Option (CNF.Clause Pos)) :=
+    cnf.clauses.map fun clause => some <| ⟨clause.literals.map fun (atom, pol) => (⟨atom + 1, by omega⟩, pol)⟩
+
+end Std.Tactic.BVDecide.LRAT.NewInternal
